theories/aneris_lang/program_logic/aneris_adequacy.v
@@ -8,11 +8,12 @@ Definition aneris_adequate (e : base_lang.expr) (ip : ip_address) (σ : state)
            (φ : base_lang.val → Prop) :=
   adequate NotStuck (mkExpr ip e) σ (λ v _, ∃ w, v = mkVal ip w ∧ φ w).
 
-Theorem adequacy `{anerisPreG Σ} IPs A e ip σ φ :
+Theorem adequacy `{anerisPreG Σ} IPs A e ip σ φ (ports : gset port) :
   (∀ `{anerisG Σ}, ⊢ |={⊤}=> ∃ (f : socket_address → socket_interp Σ),
      fixed A -∗ ([∗ set] a ∈ A, a ⤇ (f a)) -∗
      ([∗ set] i ∈ IPs, free_ip i) -∗
      WP e @[ip] ⊤ {{ v, ⌜φ v⌝ }}) →
+  ports ≠ ∅ →
   ip ∉ IPs →
   dom (gset ip_address) (state_ports_in_use σ) = IPs →
   (∀ ip, ip ∈ IPs → state_ports_in_use σ !! ip = Some ∅) →
@@ -22,7 +23,7 @@ Theorem adequacy `{anerisPreG Σ} IPs A e ip σ φ :
   state_ms σ = ∅ →
   aneris_adequate e ip σ φ.
 Proof.
-  intros Hwp Hipdom Hpiiu Hip Hfixdom Hste Hsce Hmse.
+  intros Hwp Hps Hipdom Hpiiu Hip Hfixdom Hste Hsce Hmse.
   eapply adequacy; [|done..].
   intros dg.
   iMod (Hwp dg) as (f) "Hwp".
@@ -33,12 +34,13 @@ Proof.
   eauto.
 Qed.
 
-Theorem adequacy_hoare `{anerisPreG Σ} IPs A e σ φ ip :
+Theorem adequacy_hoare `{anerisPreG Σ} IPs A e σ φ ip (ports : gset port) :
   (∀ `{anerisG Σ}, ⊢ ∃ (f : socket_address → socket_interp Σ),
       {{{ fixed A ∗ ([∗ set] a ∈ A, a ⤇ (f a)) ∗ ([∗ set] ip ∈ IPs, free_ip ip) }}}
           e @[ip]
       {{{ v, RET v; ⌜φ v⌝ }}}) →
   ip ∉ IPs →
+  ports ≠ ∅ →
   dom (gset ip_address) (state_ports_in_use σ) = IPs →
   (∀ i, i ∈ IPs → state_ports_in_use σ !! i = Some ∅) →
   (∀ a, a ∈ A → ip_of_address a ∈ IPs) →
@@ -47,7 +49,7 @@ Theorem adequacy_hoare `{anerisPreG Σ} IPs A e σ φ ip :
   state_ms σ = ∅ →
   aneris_adequate e ip σ φ.
 Proof.
-  intros Hwp ???????.
+  intros Hwp ????????.
   eapply adequacy; [|done..].
   intros ?. iModIntro.
   iDestruct Hwp as (f) "#Hwp".
